qed evidServLink.check(). adjust code to add bounds check

src/program_proof/pav/evidence.v
@@ -10,12 +10,31 @@ Section evidence.
 Context `{!heapGS Σ, !pavG Σ}.
 
 Definition is_signedLink pk (obj : signedLink.t) link : iProp Σ :=
-  is_link obj.(signedLink.epoch) obj.(signedLink.prevLink)
+  "#His_ln" ∷ is_link obj.(signedLink.epoch) obj.(signedLink.prevLink)
     obj.(signedLink.dig) link ∗
-  is_sig pk (servSepLink.encodesF (servSepLink.mk link)) obj.(signedLink.sig).
+  "#His_sig" ∷ is_sig pk (servSepLink.encodesF (servSepLink.mk link)) obj.(signedLink.sig).
+
+Lemma is_signedLink_agree_link pk obj link0 link1 :
+  is_signedLink pk obj link0 -∗
+  is_link obj.(signedLink.epoch) obj.(signedLink.prevLink)
+    obj.(signedLink.dig) link1 -∗
+  ⌜ link0 = link1 ⌝.
+Proof.
+  iIntros "H #His_ln'". iNamed "H".
+  by iDestruct (is_link_func (_,_,_) with "His_ln His_ln'") as %<-.
+Qed.
+
+Lemma is_signedLink_agree_obj pk0 pk1 obj link0 link1 :
+  is_signedLink pk0 obj link0 -∗
+  is_signedLink pk1 obj link1 -∗
+  ⌜ link0 = link1 ⌝.
+Proof.
+  iIntros "#His_sigLn0 H1". iNamedSuffix "H1" "1".
+  by iDestruct (is_signedLink_agree_link with "His_sigLn0 His_ln1") as %<-.
+Qed.
 
 Definition is_signedPut pk (obj : signedPut.t) : iProp Σ :=
-  is_sig
+  "#His_sig" ∷ is_sig
     pk
     (servSepPut.encodesF (servSepPut.mk
       obj.(signedPut.epoch) obj.(signedPut.id) obj.(signedPut.val)))
@@ -23,27 +42,28 @@ Definition is_signedPut pk (obj : signedPut.t) : iProp Σ :=
 
 Definition is_evidServLink pk (obj : evidServLink.t) : iProp Σ :=
   ∃ link0 link1,
-  is_signedLink pk (obj.(evidServLink.sigLn0)) link0 ∗
-  is_signedLink pk (obj.(evidServLink.sigLn1)) link1 ∗
+  "#His_sigLn0" ∷ is_signedLink pk (obj.(evidServLink.sigLn0)) link0 ∗
+  "#His_sigLn1" ∷ is_signedLink pk (obj.(evidServLink.sigLn1)) link1 ∗
   let epoch0 := obj.(evidServLink.sigLn0).(signedLink.epoch) in
   let epoch1 := obj.(evidServLink.sigLn1).(signedLink.epoch) in
   let prevLink1 := obj.(evidServLink.sigLn1).(signedLink.prevLink) in
-  ⌜ (epoch0 = epoch1 ∧ link0 ≠ link1)
-    ∨
-    (epoch0 = word.sub epoch1 (W64 1) ∧ link0 ≠ prevLink1) ⌝.
+  (* use nat equality for off-by-one case to prevent underflow
+  and capture >= 0 requirement. *)
+  "%Hneq_links" ∷ ⌜ (epoch0 = epoch1 ∧ link0 ≠ link1) ∨
+    (S (uint.nat epoch0) = uint.nat epoch1 ∧ link0 ≠ prevLink1) ⌝.
 
 Definition is_evidServPut pk (obj : evidServPut.t) : iProp Σ :=
   ∃ link,
-  is_signedLink pk (obj.(evidServPut.sigLn)) link ∗
-  is_signedPut pk (obj.(evidServPut.sigPut)) ∗
-  is_merkle_proof
+  "#His_sigLn" ∷ is_signedLink pk (obj.(evidServPut.sigLn)) link ∗
+  "#His_sigPut" ∷ is_signedPut pk (obj.(evidServPut.sigPut)) ∗
+  "#His_proof" ∷ is_merkle_proof
     obj.(evidServPut.proof)
     obj.(evidServPut.sigPut).(signedPut.id)
     obj.(evidServPut.val)
     obj.(evidServPut.sigLn).(signedLink.dig) ∗
   let epochLn := obj.(evidServPut.sigLn).(signedLink.epoch) in
   let epochPut := obj.(evidServPut.sigPut).(signedPut.epoch) in
-  ⌜ epochLn = epochPut ⌝.
+  "%Heq_epochs" ∷ ⌜ epochLn = epochPut ⌝.
 
 Lemma wp_signedLink_check ptr_sigLn sigLn sl_pk pk γ d0 :
   {{{
@@ -55,22 +75,20 @@ Lemma wp_signedLink_check ptr_sigLn sigLn sl_pk pk γ d0 :
   {{{
     sl_link (link : list w8) (err : bool), RET (slice_val sl_link, #err);
     "Hown_sigLn" ∷ signedLink.own ptr_sigLn sigLn ∗
-  "Hsl_pk" ∷ own_slice_small sl_pk byteT d0 pk ∗
-    "Hsl_ln" ∷ own_slice_small sl_link byteT DfracDiscarded link ∗
+    "Hsl_pk" ∷ own_slice_small sl_pk byteT d0 pk ∗
+    "#Hsl_ln" ∷ own_slice_small sl_link byteT DfracDiscarded link ∗
     (* in no err case, this lets us learn enough about the link
     to tie down err cond. *)
-    "His_ln" ∷ is_link sigLn.(signedLink.epoch) sigLn.(signedLink.prevLink)
+    "#His_ln" ∷ is_link sigLn.(signedLink.epoch) sigLn.(signedLink.prevLink)
       sigLn.(signedLink.dig) link ∗
-    "Herr" ∷ (is_signedLink pk sigLn link ∗-∗ ⌜ err = false ⌝)
+    "Hgenie" ∷ (is_signedLink pk sigLn link ∗-∗ ⌜ err = false ⌝)
   }}}.
 Proof.
   rewrite /signedLink__check.
   iIntros (Φ) "H HΦ". iNamed "H". iNamed "Hown_sigLn".
 
   (* encode link preimg. *)
-  wp_loadField.
-  wp_loadField.
-  wp_loadField.
+  do 3 wp_loadField.
   wp_apply wp_allocStruct; [val_ty|].
   iIntros (?) "Hptr_pre".
   iDestruct (struct_fields_split with "Hptr_pre") as "H".
@@ -118,373 +136,212 @@ Proof.
   destruct ok; iIntros "!>"; iSplit.
   { naive_solver. }
   3: { by iIntros "%". }
-  - iDestruct "His_sig" as "[_ His_sig]".
-    by iDestruct ("His_sig" with "[]") as "$".
-  - iIntros "[_ His_sig']".
-    iDestruct "His_sig" as "[His_sig _]".
-    by iDestruct ("His_sig" with "His_sig'") as %?.
+  - iDestruct "Hgenie" as "[_ Hgenie]".
+    by iDestruct ("Hgenie" with "[]") as "$".
+  - iNamedSuffix 1 "'".
+    iDestruct "Hgenie" as "[Hgenie _]".
+    by iDestruct ("Hgenie" with "His_sig'") as %?.
 Qed.
 
 Lemma wp_evidServLink_check ptr_evid evid sl_pk pk γ d0 :
   {{{
-    evidServLink.own ptr_evid evid ∗
-    own_slice_small sl_pk byteT d0 pk ∗
-    is_pk pk (serv_sigpred γ)
+    "Hown_evid" ∷ evidServLink.own ptr_evid evid ∗
+    "Hsl_pk" ∷ own_slice_small sl_pk byteT d0 pk ∗
+    "#His_pk" ∷ is_pk pk (serv_sigpred γ)
   }}}
   evidServLink__check #ptr_evid (slice_val sl_pk)
   {{{
     (err : bool), RET #err;
-    evidServLink.own ptr_evid evid ∗
-    own_slice_small sl_pk byteT d0 pk ∗
-    (is_evidServLink pk evid -∗ ⌜ err = false ⌝) ∗
-    if negb err then
-      False ∗
-      is_evidServLink pk evid
-    else True
+    "Hown_evid" ∷ evidServLink.own ptr_evid evid ∗
+    "Hsl_pk" ∷ own_slice_small sl_pk byteT d0 pk ∗
+    "Hgenie" ∷ (is_evidServLink pk evid ∗-∗ ⌜ err = false ⌝) ∗
+    "Herr" ∷ if negb err then False else True
   }}}.
 Proof.
   rewrite /evidServLink__check.
-  iIntros (Φ) "((%&%& HsigLn0 & Hptr_sigLn0 & HsigLn1 & Hptr_sigLn1)
-    & Hsl_pk & #His_pk) HΦ".
+  iIntros (Φ) "H HΦ". iNamed "H". iNamed "Hown_evid".
 
   (* check signed links. *)
   wp_loadField.
-  wp_apply (wp_signedLink_check with "[$HsigLn0 $Hsl_pk $His_pk]").
-  iIntros (sl_link0 link0 err0)
-    "(HsigLn0 & Hsl_pk & Hsl_link0 & #His_conn0 & Hgenie0 & Herr0)".
+  wp_apply (wp_signedLink_check with "[$Hown_sigLn0 $Hsl_pk $His_pk]").
+  iIntros (???). iNamedSuffix 1 "0".
   wp_if_destruct.
   (* error. first signed link didn't validate. *)
-  { iApply "HΦ". iFrame "HsigLn0 HsigLn1 ∗".
-    iIntros "!> (%&%& #(His_conn0' & His_sig0') &_&_)".
-    iDestruct (is_link_conn_agree_l with "His_conn0 His_conn0'") as %<-.
-    iDestruct ("Hgenie0" with "[$His_conn0' $His_sig0']") as %[=]. }
-  iDestruct "Herr0" as "#His_sigLn0".
+  { iApply "HΦ". iFrame "Hown_sigLn0 Hown_sigLn1 ∗".
+    iIntros "!>". iSplit; [|done]. iSplit; [|by iIntros "%"].
+    iNamed 1.
+    iDestruct (is_signedLink_agree_link with "His_sigLn0 His_ln0") as %<-.
+    iDestruct "Hgenie0" as "[Hgenie0 _]".
+    iDestruct ("Hgenie0" with "[$]") as "$". }
+
   wp_loadField.
-  wp_apply (wp_signedLink_check with "[$HsigLn1 $Hsl_pk $His_pk]").
-  iIntros (sl_link1 link1 err1)
-    "(HsigLn1 & Hsl_pk & Hsl_link1 & #His_conn1 & Hgenie1 & Herr1)".
+  wp_apply (wp_signedLink_check with "[$Hown_sigLn1 $Hsl_pk0 $His_pk]").
+  iIntros (???). iNamedSuffix 1 "1".
   wp_if_destruct.
   (* error. second signed link didn't validate. *)
-  { iApply "HΦ". iFrame "HsigLn0 HsigLn1 ∗".
-    iIntros "!> (%&%&_& #(His_conn1' & His_sig1') &_)".
-    iDestruct (is_link_conn_agree_l with "His_conn1 His_conn1'") as %<-.
-    iDestruct ("Hgenie1" with "[$His_conn1' $His_sig1']") as %[=]. }
-  iDestruct "Herr1" as "#His_sigLn1".
+  { iApply "HΦ". iFrame "Hown_sigLn0 Hown_sigLn1 ∗".
+    iIntros "!>". iSplit; [|done]. iSplit; [|by iIntros "%"].
+    iNamed 1.
+    iDestruct (is_signedLink_agree_link with "His_sigLn1 His_ln1") as %<-.
+    iDestruct "Hgenie1" as "[Hgenie1 _]".
+    iDestruct ("Hgenie1" with "[$]") as "$". }
 
-  (* check that links actually differ. *)
-  iDestruct "HsigLn0" as "(%&%&%&%&%&%& Hptr_epoch0 & Hptr_prevLink0 &
-    Hsl_prevLink0 & Hptr_dig0 & Hsl_dig0 & Hptr_sig0 & Hsl_sig0)".
-  iDestruct "HsigLn1" as "(%&%&%&%&%&%& Hptr_epoch1 & Hptr_prevLink1 &
-    Hsl_prevLink1 & Hptr_dig1 & Hsl_dig1 & Hptr_sig1 & Hsl_sig1)".
-  wp_loadField.
-  wp_loadField.
-  wp_loadField.
-  wp_loadField.
+  iDestruct "Hgenie0" as "[_ Hgenie0]".
+  iDestruct ("Hgenie0" with "[]") as "#His_sigLn0"; [done|].
+  iDestruct "Hgenie1" as "[_ Hgenie1]".
+  iDestruct ("Hgenie1" with "[]") as "#His_sigLn1"; [done|].
+
+  (* case: link epochs equal and links differ. *)
+  iNamedSuffix "Hown_sigLn0" "0". iNamedSuffix "Hown_sigLn1" "1".
+  do 4 wp_loadField.
   wp_if_destruct; move: Heqb1 => Heq_epoch0.
-  {
-    wp_apply (wp_BytesEqual with "[$Hsl_link0 $Hsl_link1]").
-    iIntros "[Hsl_link0 Hsl_link1]".
+  { (* epochs equal. *)
+    wp_apply (wp_BytesEqual with "[]"); [iFrame "#"|].
+    iIntros "_".
     case_bool_decide as Heq_links; iApply "HΦ".
-    -
-      (* error. links shouldn't be equal. *)
+    - (* error. links same. *)
+      iFrame "Hptr_sigLn0 ∗". iSplit; [|done]. iSplit; [|by iIntros "%"].
+      iNamedSuffix 1 "'".
+      iDestruct (is_signedLink_agree_obj with "His_sigLn0 His_sigLn0'") as %<-.
+      iDestruct (is_signedLink_agree_obj with "His_sigLn1 His_sigLn1'") as %<-.
+
+      iPureIntro.
+      destruct Hneq_links' as [[_ ?] | [Heq _]]; [done|].
+      rewrite Heq_epoch0 in Heq. lia.
+    - (* no error. links differ. *)
       iFrame "Hptr_sigLn0 ∗".
-      (* TODO: not sure why iFrame doesn't handle the True here,
-      even tho it does above. *)
-      iSplit; [|done].
-
-      iIntros "(%&%& #(His_conn0' &_) & #(His_conn1' &_) & %Heq_links')".
-      iDestruct (is_link_conn_agree_l with "His_conn0 His_conn0'") as %<-.
-      iDestruct (is_link_conn_agree_l with "His_conn1 His_conn1'") as %<-.
-
-      iPureIntro.
-      destruct Heq_links' as [[_ ?] | [Heq _]]; [done|].
-      rewrite Heq_epoch0 in Heq.
-      assert (∀ (x : w64), x ≠ word.sub x (W64 1)) as ?.
-      { intros ? H%(f_equal (word.sub x)). by ring_simplify in H. }
-      naive_solver.
-    -
-      (* no error. derive contra from two diff signed links at same epoch. *)
-      iAssert (is_evidServLink pk evid) as "His_evid".
-      { iFrame "#". naive_solver. }
-      iFrame "Hptr_sigLn0 ∗#".
-      iSplit; [naive_solver|].
-      iClear "His_evid ∗".
-
-      (* extract lookups from sigs. *)
-      iDestruct "His_sigLn0" as "(_ & His_sig0)".
-      iDestruct "His_sigLn1" as "(_ & His_sig1)".
-      iDestruct (is_sig_to_pred with "His_pk His_sig0") as "{His_sig0} HP0".
-      iDestruct (is_sig_to_pred with "His_pk His_sig1") as "{His_pk His_sig1} HP1".
-      iDestruct (get_serv_sigpred_link with "HP0") as "{HP0} HP0".
-      iDestruct (get_serv_sigpred_link with "HP1") as "{HP1} HP1".
-      iDestruct "HP0" as "(%&%&%&%& His_comm_st0 & His_conn0' & %Hlook0)".
-      iDestruct "HP1" as "(%&%&%&%& His_comm_st1 & His_conn1' & %Hlook1)".
-      iDestruct (is_link_conn_agree_r with "His_conn0 His_conn0'") as %(<-&<-&<-).
-      iDestruct (is_link_conn_agree_r with "His_conn1 His_conn1'") as %(<-&<-&<-).
-      iDestruct (is_committed_state_links_prefix with "His_comm_st0 His_comm_st1")
-        as %Hpref.
+      iSplit.
+      { iSplit; [naive_solver|].
+        iIntros "_". iFrame "#". by iLeft. }
+      iClear "His_ln0 His_ln1 Hsl_ln0 Hsl_ln1".
+      iNamedSuffix "His_sigLn0" "0". iNamedSuffix "His_sigLn1" "1".
+      (* TODO: maybe combine below steps into lemma.
+      all the way from is_pk is_sig to inner link sigpred.
+      in link sigpred, is_ln should be in outer def.
+      from link sig, extract pred. *)
+      iDestruct (is_sig_to_pred with "His_pk His_sig0") as "#HP0".
+      iDestruct (is_sig_to_pred with "His_pk His_sig1") as "#HP1".
+      iDestruct (serv_sigpred_know_link with "HP0") as "{HP0} HP0".
+      iDestruct (serv_sigpred_know_link with "HP1") as "{HP1} HP1".
+      iNamedSuffix "HP0" "0'". iNamedSuffix "HP1" "1'".
+      iDestruct (is_link_inj (_,_,_) (_,_,_) with "His_ln0 His_ln0'") as %H. inv H.
+      iDestruct (is_link_inj (_,_,_) (_,_,_) with "His_ln1 His_ln1'") as %H. inv H.
+      iDestruct (is_com_st_links_prefix with "His_com0' His_com1'") as %Hpref.
 
       iPureIntro.
-      rewrite -Heq_epoch0 in Hlook1.
+      rewrite -Heq_epoch0 in Hlook_ln1'.
       destruct Hpref as [Hpref | Hpref].
-      { pose proof (prefix_lookup_Some _ _ _ _ Hlook0 Hpref) as ?. naive_solver. }
-      { pose proof (prefix_lookup_Some _ _ _ _ Hlook1 Hpref) as ?. naive_solver. }
+      (* core reason: link0 differs from link1.
+      they're at the same epoch of prefixed lists. *)
+      { pose proof (prefix_lookup_Some _ _ _ _ Hlook_ln0' Hpref) as ?. naive_solver. }
+      { pose proof (prefix_lookup_Some _ _ _ _ Hlook_ln1' Hpref) as ?. naive_solver. }
   }
-  wp_loadField.
-  wp_loadField.
-  wp_loadField.
-  wp_loadField.
+
+  (* case: S epoch0 = epoch1 and link0 differs from prevLink1. *)
+  wp_apply (wp_and' with "[-] [] []"); [iNamedAccu|..].
+  { iNamed 1. do 2 wp_loadField. wp_pures. by iFrame "∗#". }
+  { iNamed 1. iIntros "_". do 4 wp_loadField. wp_pures. by iFrame "∗#". }
+  iNamed 1.
+
+  (* we take two w64 props and show that they're equal to a nat prop.
+  the latter can be more easily used in list lemmas. *)
+  assert (
+    bool_decide
+    ((uint.Z (W64 0) < uint.Z evid.(evidServLink.sigLn1).(signedLink.epoch))%Z
+      ∧ (#evid.(evidServLink.sigLn0).(signedLink.epoch) =
+        #(LitInt (word.sub evid.(evidServLink.sigLn1).(signedLink.epoch) (W64 1))))%V) =
+    bool_decide (S (uint.nat evid.(evidServLink.sigLn0).(signedLink.epoch)) =
+      uint.nat evid.(evidServLink.sigLn1).(signedLink.epoch))) as ->.
+  { replace (uint.Z (W64 0)) with (0%Z) by word.
+    case_bool_decide as H10; case_bool_decide as H11.
+    { naive_solver. }
+    #[local] Ltac Zify.zify_post_hook ::= Z.div_mod_to_equations.
+    { destruct H10 as [H9 H10].
+      apply inv_litint in H10.
+      rewrite H10 word.unsigned_sub /word.wrap in H11. word. }
+    { apply Classical_Prop.not_and_or in H10 as [H10 | H10]; [lia|].
+      apply u64_val_ne in H10.
+      rewrite word.unsigned_sub /word.wrap in H10. word. }
+    { naive_solver. } }
+
   wp_if_destruct; move: Heqb1 => Heq_epoch1.
-  {
-    wp_loadField.
-    wp_loadField.
-    wp_apply (wp_BytesEqual with "[$Hsl_link0 $Hsl_prevLink1]").
-    iIntros "[Hsl_link0 Hsl_prevLink1]".
+  { (* S epoch0 = epoch1. *)
+    do 2 wp_loadField.
+    wp_apply (wp_BytesEqual with "[Hsl_prevLink1]"); [iFrame "∗#"|].
+    iIntros "[_ Hsl_prevLink1]".
     case_bool_decide as Heq_links; iApply "HΦ".
-    -
-      (* error. links shouldn't be equal. *)
+    - (* error. links same. *)
+      iFrame "Hptr_sigLn0 ∗". iSplit; [|done]. iSplit; [|by iIntros "%"].
+      iNamedSuffix 1 "'".
+      iDestruct (is_signedLink_agree_obj with "His_sigLn0 His_sigLn0'") as %<-.
+      iDestruct (is_signedLink_agree_obj with "His_sigLn1 His_sigLn1'") as %<-.
+
+      iPureIntro.
+      destruct Hneq_links' as [[Heq _] | [_ ?]]; [|done].
+      rewrite Heq in Heq_epoch0. naive_solver.
+    - (* no error. links differ. *)
       iFrame "Hptr_sigLn0 ∗".
-      (* TODO: not sure why iFrame doesn't handle the True here,
-      even tho it does above. *)
-      iSplit; [|done].
+      iSplit.
+      { iSplit; [naive_solver|].
+        iIntros "_". iFrame "#". naive_solver. }
+      iClear "His_ln0 His_ln1 Hsl_ln0 Hsl_ln1".
+      iNamedSuffix "His_sigLn0" "0". iNamedSuffix "His_sigLn1" "1".
+      iDestruct (is_sig_to_pred with "His_pk His_sig0") as "#HP0".
+      iDestruct (is_sig_to_pred with "His_pk His_sig1") as "#HP1".
+      iDestruct (serv_sigpred_know_link with "HP0") as "{HP0} HP0".
+      iDestruct (serv_sigpred_know_link with "HP1") as "{HP1} HP1".
+      iNamedSuffix "HP0" "0'". iNamedSuffix "HP1" "1'".
+      iDestruct (is_link_inj (_,_,_) (_,_,_) with "His_ln0 His_ln0'") as %H. inv H.
+      iDestruct (is_link_inj (_,_,_) (_,_,_) with "His_ln1 His_ln1'") as %H. inv H.
+      iDestruct (is_com_st_links_prefix with "His_com0' His_com1'") as %Hpref.
 
-      iIntros "(%&%& #(His_conn0' &_) & #(His_conn1' &_) & %Heq_links')".
-      iDestruct (is_link_conn_agree_l with "His_conn0 His_conn0'") as %<-.
-      iDestruct (is_link_conn_agree_l with "His_conn1 His_conn1'") as %<-.
+      iClear "His_ln0' His_ln1' His_sig0 His_sig1".
+      opose proof (lookup_lt_is_Some_2 com_st0.(links)
+        (uint.nat evid.(evidServLink.sigLn0).(signedLink.epoch)) _)
+        as [? Hlook_prevLn1].
+      { opose proof (lookup_lt_is_Some_1 _ _ _) as ?.
+        { eexists. exact Hlook_ln1'. }
+        lia. }
+      iNamedSuffix "His_com1'" "1".
+      iDestruct (big_sepL_lookup with "Hlinks1") as "His_chain_prevLn1".
+      { exact Hlook_prevLn1. }
+      iDestruct (big_sepL_lookup with "Hlinks1") as "His_chain_ln1".
+      { exact Hlook_ln1'. }
+
+      opose proof (lookup_lt_is_Some_2 com_st0.(digs)
+        (uint.nat evid.(evidServLink.sigLn0).(signedLink.epoch)) _) as [? Hlook_tmp].
+      { opose proof (lookup_lt_is_Some_1 _ _ _) as ?.
+        { eexists. exact Hlook_prevLn1. }
+        lia. }
+      opose proof (take_S_r _ _ _ _) as Htake_digs.
+      { exact Hlook_tmp. }
+      clear Hlook_tmp.
+      iEval (rewrite -Heq_epoch1 Htake_digs) in "His_chain_ln1".
+
+      iDestruct (is_chain_to_link with "His_chain_prevLn1 His_chain_ln1") as "His_ln1'".
+      iDestruct (is_link_inj (_,_,_) (_,_,_) with "His_ln1 His_ln1'") as %H.
+      inv H as [H1]. clear H1.
 
       iPureIntro.
-      destruct Heq_links' as [[Heq _] | [_ ?]]; [|done].
-      rewrite Heq_epoch1 in Heq.
-      assert (∀ (x : w64), x ≠ word.sub x (W64 1)) as ?.
-      { intros ? H%(f_equal (word.sub x)). by ring_simplify in H. }
-      naive_solver.
-    -
-      (* no error. derive contra from prev.link differing from curr.prevLink. *)
-      iAssert (is_evidServLink pk evid) as "His_evid".
-      { iFrame "#". naive_solver. }
-      iFrame "Hptr_sigLn0 ∗#".
-      iSplit; [naive_solver|].
-      iClear "His_evid ∗".
-
-      (* extract lookups from sigs. *)
-      iDestruct "His_sigLn0" as "(_ & His_sig0)".
-      iDestruct "His_sigLn1" as "(_ & His_sig1)".
-      iDestruct (is_sig_to_pred with "His_pk His_sig0") as "{His_sig0} HP0".
-      iDestruct (is_sig_to_pred with "His_pk His_sig1") as "{His_pk His_sig1} HP1".
-      iDestruct (get_serv_sigpred_link with "HP0") as "{HP0} HP0".
-      iDestruct (get_serv_sigpred_link with "HP1") as "{HP1} HP1".
-      iDestruct "HP0" as "(%&%&%&%& His_comm_st0 & His_conn0' & %Hlook0)".
-      iDestruct "HP1" as "(%&%&%&%& His_comm_st1 & His_conn1' & %Hlook1)".
-      iDestruct (is_link_conn_agree_r with "His_conn0 His_conn0'") as %(<-&<-&<-).
-      iDestruct (is_link_conn_agree_r with "His_conn1 His_conn1'") as %(<-&<-&<-).
-      iDestruct (is_committed_state_links_prefix with "His_comm_st0 His_comm_st1")
-        as %Hpref.
-
-      iPureIntro.
-      simpl in *.
-      rewrite Heq_epoch1 in Hlook0.
-      (*
-      Hlook0: links0 !! (epoch1 - 1) = Some link0.
-      Hlook1: links1 !! epoch1 = Some link1.
-      from Hlook1, should derive that:
-      links1 !! (epoch1 - 1) = Some prevLink1.
-
-      how?
-      from link sigpred, know that a specific link is smth.
-      also have prevLink tied into there with is_conn.
-      from committed state (binds), should be able to derive that
-      adjacent lookups tied together by conn.
-
-      binds says that prefixes of digs match up to links.
-      should be not too bad to prove:
-      is_link digs prevLink -∗
-      is_link (digs ++ [new_dig]) link -∗
-      is_link_conn prevLink new_dig link.
-      *)
       destruct Hpref as [Hpref | Hpref].
-      { pose proof (prefix_lookup_Some _ _ _ _ Hlook0 Hpref) as ?. naive_solver. }
-      { pose proof (prefix_lookup_Some _ _ _ _ Hlook1 Hpref) as ?. naive_solver. }
-
-(*
-  rewrite /evidServLink__check.
-  iIntros (Φ) "H HΦ"; iNamed "H"; iNamed "Hevid".
-
-  (* first link sig. *)
-  wp_loadField.
-  wp_loadField.
-  wp_loadField.
-  wp_apply wp_allocStruct; [val_ty|];
-    iIntros (ptr_linkSep0) "Hptr_linkSep0".
-  iDestruct (struct_fields_split with "Hptr_linkSep0") as "H";
-    iNamed "H"; iClear "tag".
-  iMod (own_slice_small_persist with "Hsl_prevLink0") as "#Hsl_prevLink0".
-  wp_apply (chainSepSome.wp_encode with "[epoch prevLink data Hsl_prevLink0 Hsl_dig0]").
-  {
-    instantiate (1:=chainSepSome.mk _ _ _).
-    rewrite /chainSepSome.own /=.
-    iExists sl_prevLink0, sl_dig0; iFrame "#∗".
-  }
-  iIntros (sl_link0Enc link0Enc) "H"; iNamed "H";
-    iRename "Hobj" into "Hptr_linkSep0";
-    iRename "Hsl_enc" into "Hsl_link0Enc";
-    rename Henc into Henc_link0.
-  wp_apply (wp_Hash with "Hsl_link0Enc");
-    iIntros (sl_link0 link0) "H"; iNamed "H";
-    iRename "Hdata" into "Hsl_link0Enc";
-    iRename "Hhash" into "Hsl_link0";
-    iRename "His_hash" into "His_hash_link0".
-  iMod (own_slice_small_persist with "Hsl_link0") as "#Hsl_link0".
-  wp_apply wp_allocStruct; [val_ty|];
-    iIntros (ptr_enc0) "Hptr_enc0".
-  iDestruct (struct_fields_split with "Hptr_enc0") as "H";
-    iNamed "H"; iClear "tag".
-  wp_apply (servSepLink.wp_encode with "[link]").
-  {
-    instantiate (1:=servSepLink.mk _).
-    rewrite /servSepLink.own /=.
-    iFrame "#∗".
-  }
-  iIntros (sl_enc0 enc0) "H"; iNamed "H";
-    iRename "Hobj" into "Hptr_enc0";
-    iRename "Hsl_enc" into "Hsl_enc0";
-    rename Henc into Henc_enc0.
-  wp_loadField.
-  wp_apply (wp_Verify with "[Hsl_enc0 Hsl_sig0]"); [iFrame "#∗"|];
-    iIntros (?) "H"; iNamed "H";
-    iRename "Hsig" into "Hsl_sig0";
-    iRename "Hmsg" into "Hsl_enc0";
-    iRename "HP" into "Hsigpred0".
-  destruct ok.
-  2: { wp_pures. by iApply "HΦ". }
-
-  (* second link sig. *)
-  wp_loadField.
-  wp_loadField.
-  wp_loadField.
-  wp_apply wp_allocStruct; [val_ty|];
-    iIntros (ptr_linkSep1) "Hptr_linkSep1".
-  iDestruct (struct_fields_split with "Hptr_linkSep1") as "H";
-    iNamed "H"; iClear "tag".
-  iMod (own_slice_small_persist with "Hsl_prevLink1") as "#Hsl_prevLink1".
-  wp_apply (chainSepSome.wp_encode with "[epoch prevLink data Hsl_prevLink1 Hsl_dig1]").
-  {
-    instantiate (1:=chainSepSome.mk _ _ _).
-    rewrite /chainSepSome.own /=.
-    iExists sl_prevLink1, sl_dig1; iFrame "#∗".
-  }
-  iIntros (sl_link1Enc link1Enc) "H"; iNamed "H";
-    iRename "Hobj" into "Hptr_linkSep1";
-    iRename "Hsl_enc" into "Hsl_link1Enc";
-    rename Henc into Henc_link1.
-  wp_apply (wp_Hash with "Hsl_link1Enc");
-    iIntros (sl_link1 link1) "H"; iNamed "H";
-    iRename "Hdata" into "Hsl_link1Enc";
-    iRename "Hhash" into "Hsl_link1";
-    iRename "His_hash" into "His_hash_link1".
-  iMod (own_slice_small_persist with "Hsl_link1") as "#Hsl_link1".
-  wp_apply wp_allocStruct; [val_ty|];
-    iIntros (ptr_enc1) "Hptr_enc1".
-  iDestruct (struct_fields_split with "Hptr_enc1") as "H";
-    iNamed "H"; iClear "tag".
-  wp_apply (servSepLink.wp_encode with "[link]").
-  {
-    instantiate (1:=servSepLink.mk _).
-    rewrite /servSepLink.own /=.
-    iFrame "#∗".
-  }
-  iIntros (sl_enc1 enc1) "H"; iNamed "H";
-    iRename "Hobj" into "Hptr_enc1";
-    iRename "Hsl_enc" into "Hsl_enc1";
-    rename Henc into Henc_enc1.
-  wp_loadField.
-  wp_apply (wp_Verify with "[Hsl_enc1 Hsl_sig1]"); [iFrame "#∗"|];
-    iIntros (?) "H"; iNamed "H";
-    iRename "Hsig" into "Hsl_sig1";
-    iRename "Hmsg" into "Hsl_enc1".
-    iRename "HP" into "Hsigpred1".
-  destruct ok.
-  2: { wp_pures. by iApply "HΦ". }
-
-  (* epochs are equal. *)
-  wp_loadField.
-  wp_loadField.
-  wp_if_destruct; rename Heqb into Hepoch_eq.
-  1: {
-    (* TODO: why does:
-      wp_apply (wp_BytesEqual "[$Hsl_link0 $Hsl_link1]").
-      not work? *)
-    wp_apply wp_BytesEqual; [iFrame "#"|].
-    iIntros "_".
-    case_bool_decide; [by iApply "HΦ"|]; rename H into Hlink_ne.
-    destruct hon; [|by iApply "HΦ"].
-    iDestruct "Hsigpred0" as "[[%sepLink0 [%Henc_link0' Hsigpred0]] | [% [%Henc_put _]]]".
-    2: { exfalso. eauto using servSep. }
-    iDestruct "Hsigpred1" as "[[%sepLink1 [%Henc_link1' Hsigpred1]] | [% [%Henc_put _]]]".
-    2: { exfalso. eauto using servSep. }
-
-    (* open binding, apply val divergence to prove false. *)
-    iExFalso.
-    rewrite ->Henc_link0' in Henc_enc0;
-      apply servSepLink.inj in Henc_enc0 as ->.
-    rewrite ->Henc_link1' in Henc_enc1;
-      apply servSepLink.inj in Henc_enc1 as ->.
-    iDestruct "Hsigpred0" as (epoch0 prevLink0 dig0) "H"; iNamed "H";
-      iRename "Hbind" into "Hbind0";
-      iClear "HidxPrev";
-      iRename "HidxCurr" into "HidxCurr0".
-    iDestruct "Hsigpred1" as (epoch1 prevLink1 dig1) "H"; iNamed "H";
-      iRename "Hbind" into "Hbind1";
-      iClear "HidxPrev";
-      iRename "HidxCurr" into "HidxCurr1".
-    iDestruct (hash_inj with "[$His_hash_link0] [$Hbind0]") as %->.
-    iDestruct (hash_inj with "[$His_hash_link1] [$Hbind1]") as %->.
-    apply chainSepSome.inj in Henc_link0 as [=]; subst.
-    apply chainSepSome.inj in Henc_link1 as [=]; subst.
-    iEval (rewrite Hepoch_eq) in "HidxCurr0".
-    iDestruct (mono_list_idx_agree with "[$HidxCurr0] [$HidxCurr1]") as %[=].
-    done.
+      (* core reason: link0 differs from prevLink1.
+      they're at the same epoch of prefixed lists. *)
+      { pose proof (prefix_lookup_Some _ _ _ _ Hlook_ln0' Hpref) as ?. naive_solver. }
+      { pose proof (prefix_lookup_Some _ _ _ _ Hlook_prevLn1 Hpref) as ?. naive_solver. }
   }
 
-  (* epochs are off by one, but apart from that,
-     almost same analysis as epoch equals case. *)
-  wp_loadField.
-  wp_loadField.
-  wp_if_destruct; rename Heqb into Hepoch_off_eq.
-  1: {
-    wp_loadField.
-    wp_apply wp_BytesEqual; [iFrame "#"|].
-    iIntros "_".
-    case_bool_decide; [by iApply "HΦ"|]; rename H into Hlink_ne.
-    destruct hon; [|by iApply "HΦ"].
-    iDestruct "Hsigpred0" as "[[%sepLink0 [%Henc_link0' Hsigpred0]] | [% [%Henc_put _]]]".
-    2: { exfalso. eauto using servSep. }
-    iDestruct "Hsigpred1" as "[[%sepLink1 [%Henc_link1' Hsigpred1]] | [% [%Henc_put _]]]".
-    2: { exfalso. eauto using servSep. }
+  (* failed both if conds, so no valid evid. *)
+  iApply "HΦ".
+  iFrame "Hptr_sigLn0 ∗". iIntros "!>". iSplit; [|done]. iSplit; [|by iIntros "%"].
+  iNamedSuffix 1 "'".
+  iDestruct (is_signedLink_agree_obj with "His_sigLn0 His_sigLn0'") as %<-.
+  iDestruct (is_signedLink_agree_obj with "His_sigLn1 His_sigLn1'") as %<-.
 
-    iExFalso.
-    rewrite ->Henc_link0' in Henc_enc0;
-      apply servSepLink.inj in Henc_enc0 as ->.
-    rewrite ->Henc_link1' in Henc_enc1;
-      apply servSepLink.inj in Henc_enc1 as ->.
-    iDestruct "Hsigpred0" as (epoch0 prevLink0 dig0) "H"; iNamed "H";
-      iRename "Hbind" into "Hbind0";
-      iClear "HidxPrev";
-      iRename "HidxCurr" into "HidxCurr0".
-    iDestruct "Hsigpred1" as (epoc10 prevLink1 dig1) "H"; iNamed "H";
-      iRename "Hbind" into "Hbind1";
-      iRename "HidxPrev" into "HidxPrev1";
-      iClear "HidxCurr".
-    iDestruct (hash_inj with "[$His_hash_link0] [$Hbind0]") as %->.
-    iDestruct (hash_inj with "[$His_hash_link1] [$Hbind1]") as %->.
-    apply chainSepSome.inj in Henc_link0 as [=]; subst.
-    apply chainSepSome.inj in Henc_link1 as [=]; subst.
-    iEval (rewrite Hepoch_off_eq) in "HidxCurr0".
-    iDestruct (mono_list_idx_agree with "[$HidxCurr0] [$HidxPrev1]") as %[=].
-    done.
-  }
-  by iApply "HΦ".
+  iPureIntro.
+  destruct Hneq_links' as [[Heq _] | [Heq _]].
+  { by rewrite Heq in Heq_epoch0. }
+  { by rewrite Heq in Heq_epoch1. }
 Qed.
-*)
 
 Lemma wp_evidServPut_check ptr_evid evid sl_pk pk γ d0 :
   {{{
